ectx_lang.v
@@ -1,0 +1,269 @@
+Require Import Arith Ssreflect.ssreflect Ssreflect.ssrfun.
+Require Import world_prop world_prop_recdom core_lang lang iris_core iris_plog iris_ht_rules.
+Require Import ModuRes.RA ModuRes.SPred ModuRes.BI ModuRes.PreoMet ModuRes.Finmap ModuRes.RAConstr ModuRes.CMRA.
+
+Set Bullet Behavior "Strict Subproofs".
+
+(** This file defines an interface for languages with evaluation contexts, and shows that they have a Bind rule. *)
+Module Type ECTX_LANG.
+
+  (******************************************************************)
+  (** ** Syntax, machine state, and atomic reductions **)
+  (******************************************************************)
+
+  (** Expressions and values **)
+  Parameter expr : Type.
+
+  Parameter is_value : expr -> Prop.
+  Definition value : Type := {e: expr | is_value e}.
+  Parameter is_value_dec : forall e, is_value e + ~is_value e.
+
+  (** Evaluation contexts **)
+  Parameter ectx : Type.
+  Parameter empty_ctx : ectx.
+  Parameter comp_ctx : ectx -> ectx -> ectx.
+  Parameter fill : ectx -> expr -> expr.
+(*
+	All of
+		comp_ctx_assoc
+		comp_ctx_inj_r
+		comp_ctx_emp_r
+	arise only in the proof of
+
+		step_same_ctx K K' e e' :
+			fill K e = fill K' e' ->
+			reducible e  ->
+			reducible e' ->
+			K = K'.
+
+	Moreover, comp_ctx_positive gets used only in step_same_ctx
+	and
+
+		
+	
+	It might be simpler to (prove and) assume these two rather
+	than those four.
+*)
+(*  Axiom comp_ctx_emp_r : forall K,
+    comp_ctx K empty_ctx = K.
+  Axiom comp_ctx_assoc : forall K0 K1 K2,
+    comp_ctx K0 (comp_ctx K1 K2) = comp_ctx (comp_ctx K0 K1) K2.
+  Axiom comp_ctx_inj_r : forall K K1 K2,
+    comp_ctx K K1 = comp_ctx K K2 -> K1 = K2.
+  Axiom comp_ctx_positive : forall K1 K2,
+    comp_ctx K1 K2 = empty_ctx -> K1 = empty_ctx /\ K2 = empty_ctx. *)
+
+  Axiom fill_empty : forall e, fill empty_ctx e = e.
+  Axiom fill_comp  : forall K1 K2 e, fill K1 (fill K2 e) = fill (comp_ctx K1 K2) e.
+  Axiom fill_inj_r  : forall K e1 e2, fill K e1 = fill K e2 -> e1 = e2.
+  Axiom fill_value : forall K e, is_value (fill K e) -> is_value e.
+
+  (** Shared machine state (e.g., the heap) **)
+  Parameter state : Type.
+
+  (** Primitive (single thread) machine configurations **)
+  Definition prim_cfg : Type := (expr * state)%type.
+
+  (** The primitive atomic stepping relation **)
+  Parameter prim_step : prim_cfg -> prim_cfg -> option expr -> Prop.
+  
+  (** Some derived notions. **)
+  Definition reducible e: Prop :=
+    exists sigma cfg' ef, prim_step (e, sigma) cfg' ef.
+
+  Definition stuck (e : expr) : Prop :=
+    forall K e',
+      e = fill K e' ->
+      ~reducible e'.
+
+  (** Atomic expressions **)
+  Parameter atomic : expr -> Prop.
+
+  (** Things ought to make sense. *)
+  Axiom values_stuck :
+    forall e, is_value e -> stuck e.
+
+  (* When something does a step, and another decomposition of the same
+     expression has a non-value e in the hole, then K is a left
+     sub-context of K' - in other words, e also contains the reducible
+     expression *)
+  Axiom step_by_value :
+    forall K K' e e',
+      fill K e = fill K' e' ->
+      reducible e' ->
+      ~ is_value e ->
+      exists K'', K' = comp_ctx K K''.
+
+  Axiom atomic_not_value :
+    forall e, atomic e -> ~is_value e.
+
+  Axiom atomic_step: forall e σ e' σ' ef,
+                       atomic e ->
+                       prim_step (e, σ) (e', σ') ef ->
+                       is_value e'.
+
+  (* Atomics must not contain evaluation positions. *)
+  Axiom atomic_fill: forall e K,
+			atomic (fill K e) ->
+			~ is_value e ->
+			K = empty_ctx.
+End ECTX_LANG.
+
+Module EctxCoreLang (C: ECTX_LANG) <: CORE_LANG.
+
+  Definition expr := C.expr.
+  Definition is_value := C.is_value.
+  Definition value := C.value.
+  Definition is_value_dec := C.is_value_dec.
+
+  Definition state := C.state.
+  Definition prim_cfg := C.prim_cfg.
+
+  (** Some derived properties **)
+(*  Section Derived.
+    Import C.
+
+    Lemma reducible_not_value {e} :
+      reducible e -> ~is_value e.
+    Proof.
+      intros H_red H_val.
+      eapply values_stuck; try eassumption.
+      now erewrite fill_empty.
+    Qed.
+    
+(*    Lemma step_same_ctx {K K' e e'} :
+      fill K e = fill K' e' ->
+      reducible e  ->
+      reducible e' ->
+      K = K'.
+    Proof.
+      intros H_fill H_red H_red'.
+      edestruct (step_by_value K K' e e') as [K'' H_K''].
+      - assumption.
+      - assumption.
+      - now apply reducible_not_value.
+      - edestruct (step_by_value K' K e' e) as [K''' H_K'''].
+        + now symmetry.
+        + assumption.
+        + now apply reducible_not_value.
+        + subst K.
+          rewrite <- comp_ctx_assoc in H_K''.
+          assert (H_emp := comp_ctx_neut_emp_r H_K'').
+          apply comp_ctx_positive in H_emp.
+          destruct H_emp as[H_K'''_emp H_K''_emp].
+          subst K'' K'''.
+          now rewrite comp_ctx_emp_r.
+    Qed. *)
+
+  End Derived.
+*)
+
+  (** Base reduction **)
+  Definition prim_step (c1 c2: prim_cfg) (ef: option expr) :=
+    match c1, c2 with
+    | (e1, σ1), (e2, σ2) => exists K e1' e2', e1 = C.fill K e1' /\ e2 = C.fill K e2' /\
+                                              C.prim_step (e1', σ1) (e2', σ2) ef
+    end.
+
+  Definition reducible e: Prop :=
+    exists sigma cfg' ef, prim_step (e, sigma) cfg' ef.
+  Definition stuck e := ~reducible e.
+
+  Lemma reducible_eq e: reducible e <-> exists K e', e = C.fill K e' /\ C.reducible e'.
+  Proof.
+    split.
+    - intros (σ & c2 & ef & Hstep). destruct c2 as [e2 σ2].
+      destruct Hstep as (K & e' & e2' & Heq1 & Heq2 & Hstep).
+      exists K e'. split; first assumption. exists σ (e2', σ2) ef.
+      assumption.
+    - intros (K & e' & Heq & Hred). destruct Hred as (σ & c2 & ef & Hred). destruct c2 as [e2 σ2].
+      exists σ (C.fill K e2, σ2) ef. exists K e' e2. split; last split; assumption || reflexivity.
+  Qed.
+
+  Lemma stuck_eq e: stuck e <-> C.stuck e.
+  Proof.
+    split; intros H1.
+    - intros K e' Heq Hred. apply H1, reducible_eq. do 2 eexists. split; eassumption.
+    - intros H. apply reducible_eq in H. destruct H as (K & e' & Heq & Hred). eapply H1; eassumption.
+  Qed.
+
+  Lemma values_stuck :
+    forall e, is_value e -> stuck e.
+  Proof.
+    intros. apply stuck_eq, C.values_stuck. assumption.
+  Qed.
+
+  (** Atomic **)
+  Definition atomic := C.atomic.
+
+  Lemma atomic_not_value :
+    forall e, atomic e -> ~is_value e.
+  Proof.
+    exact C.atomic_not_value.
+  Qed.
+
+  Lemma atomic_step: forall e σ e' σ' ef,
+      atomic e ->
+      prim_step (e, σ) (e', σ') ef ->
+      is_value e'.
+  Proof.
+    intros ? ? ? ? ? Hatomic (K & e1' & e2' & Heq1 & Heq2 & Hstep).
+    move:(C.atomic_fill e1' K). subst. case/(_ _ _)/Wrap.
+    - assumption.
+    - intros Hval. eapply C.values_stuck; [eassumption|erewrite C.fill_empty;reflexivity|].
+      do 3 eexists. eassumption.
+    - intros Heq. subst.
+      eapply C.atomic_step; first eassumption.
+      erewrite !C.fill_empty. eassumption.
+  Qed.
+
+End EctxCoreLang.
+
+Module Type ECTX_RES (RL : VIRA_T) (E : ECTX_LANG) <: CMRA_EXT_T.
+ Module C := EctxCoreLang E.
+ Include IRIS_RES RL C.
+End ECTX_RES.
+
+Module EctxRes (RL : VIRA_T) (E : ECTX_LANG) <: ECTX_RES RL E.
+  Include ECTX_RES RL E.
+End EctxRes.
+
+Module ECTX_IRIS (RL : VIRA_T) (E : ECTX_LANG) (R: ECTX_RES RL E) (WP: WORLD_PROP R).
+
+  Module Lang := EctxCoreLang E.
+  Module Res := IrisRes RL Lang.
+  Module World := WorldProp Res.
+  Module Import Core := IrisCore RL Lang Res World.
+  Module Import Plog := IrisPlog RL Lang Res World Core.
+  Module Import HTRules := IrisHTRules RL Lang Res World Core Plog.
+
+  (** We can hae bind with evaluation contexts **)
+  Lemma fill_is_fill K: IsFill (E.fill K).
+  Proof.
+    split; intros; last (split; intros; first split).
+    - eapply E.fill_value. eassumption.
+    - intros (K' & e1' & e2' & Heq1 & Heq2 & Hstep).
+      exists (E.comp_ctx K K') e1' e2'. rewrite -!E.fill_comp Heq1 Heq2.
+      split; last split; reflexivity || assumption.
+    - intros (K' & e1' & e2' & Heq1 & Heq2 & Hstep).
+      destruct (E.step_by_value _ _ _ _ Heq1) as [K'' HeqK].
+      + do 3 eexists. eassumption.
+      + assumption.
+      + exists K''. subst K'. rewrite -!E.fill_comp in Heq1, Heq2.
+        apply E.fill_inj_r in Heq1. apply E.fill_inj_r in Heq2.
+        do 2 eexists. split; last split; eassumption.
+    - destruct H0 as (K' & e1' & e2' & Heq1 & Heq2 & Hstep).
+      destruct (E.step_by_value _ _ _ _ Heq1) as [K'' HeqK].
+      + do 3 eexists. eassumption.
+      + assumption.
+      + subst K'. rewrite -E.fill_comp in Heq2.
+        eexists. eassumption.
+  Qed.
+        
+  Lemma wpBind φ K e safe m :
+    wp safe m e (plug_bind (E.fill K) safe m φ) ⊑ wp safe m (E.fill K e) φ.
+  Proof.
+    apply wpBind. apply fill_is_fill.
+  Qed.
+
+End ECTX_IRIS.
